allocator/slabs bottom-up 9/n
size_class -> slab roughly done,
to be refined:
- remove assume (pure into vprop)
- ind_llist support with nested vprops
- (later, with init) refine size_class type

src/Slabs.fst
@@ -425,7 +425,13 @@ let allocate_slot_kiss (size_class: sc)
   (slab_vprop size_class arr 0 (U32.v (nb_slots size_class)) `star` A.varray md)
   (fun r -> slab_vprop size_class arr 0 (U32.v (nb_slots size_class)) `star` A.varray md)
   (requires fun h0 -> has_free_slot size_class (A.asel md h0))
-  (ensures fun _ _ _ -> True)
+  (ensures fun h0 r h1 ->
+    let bm0 = Bitmap4.array_to_bv2 (A.asel md h0) in
+    let bm1 = Bitmap4.array_to_bv2 (A.asel md h1) in
+    let idx = Bitmap5.f #4 (G.reveal (fst r)) in
+    Seq.index bm0 idx = false /\
+    bm1 == Seq.upd bm0 idx true
+    )
   =
   let slot_pos = get_free_slot size_class md in
   Bitmap5.bm_set #(G.hide 4) md slot_pos;
@@ -450,30 +456,15 @@ unfold let p (size_class: sc)
      `star` slab_vprop size_class (f md) 0 (U32.v (nb_slots size_class))
 
 // Given a size class, return a free slot and update metadata
-#push-options "--ifuel 2 --fuel 2"
-let allocate_slab
-  (size_class: sc)
-  (slabs: SL.t U64.t)
-  : Steel
-  //(SL.t U64.t)
-  //_
-  unit
-  (SL.llist (fun _ -> emp) slabs)
-  //(fun ptr2 -> vptr slabs `star` SL.llist (fun _ -> emp) ptr2)
-  (fun _ -> SL.llist (fun _ -> emp) slabs)
-  (requires fun _ -> not (SL.is_null_t slabs))
-  (ensures fun _ _ _ -> True)
-  =
-  let n = SL.unpack_list (fun _ -> emp) slabs in
-  SL.pack_list (fun _ -> emp) slabs (SL.get_next n) (SL.get_data n);
-  return ()
-
+// TODO: add ind_llist
+// TODO: remove assume with pure predicates inside p
+//   this will yield two different versions of p
 let allocate_slab2
   (sc: sc)
   (partial_slabs: SL.t (slab_metadata))
   (empty_slabs: SL.t (slab_metadata))
   //: Steel (SL.cell (slab_metadata))
-  : Steel (SL.t slab_metadata & SL.t slab_metadata)
+  : Steel (array U8.t & (SL.t slab_metadata & SL.t slab_metadata))
   (
   SL.llist (p sc) partial_slabs
   `star`
@@ -481,82 +472,51 @@ let allocate_slab2
   )
   (
   fun r ->
-  SL.llist (p sc) (fst r)
+  SL.llist (p sc) (fst (snd r))
   `star`
-  SL.llist (p sc) (snd r)
+  SL.llist (p sc) (snd (snd r))
   )
-  (requires fun _ ->
+  (requires fun h0 ->
+    not (SL.is_null_t partial_slabs) \/
     not (SL.is_null_t empty_slabs))
-    //not (SL.is_null_t partial_slabs))
   (ensures fun _ _ _ -> True)
   =
   if SL.is_null_t partial_slabs then (
     assert (not (SL.is_null_t empty_slabs));
-    let n_old_empty_slabs = SL.unpack_list (p sc) empty_slabs in
-    let n_new_partial_slabs = SL.mk_cell partial_slabs (SL.get_data n_old_empty_slabs) in
-    write empty_slabs n_new_partial_slabs;
+    let n_empty = SL.unpack_list (p sc) empty_slabs in
+    let n_partial = SL.mk_cell partial_slabs (SL.get_data n_empty) in
+    let h = get () in
+    let md = SL.get_data n_empty in
+    assume (has_free_slot sc (A.asel md h));
+    let r = allocate_slot_kiss sc
+      (SL.get_data n_empty)
+      (f (SL.get_data n_empty)) in
+    write empty_slabs n_partial;
     slassert (
-      SL.llist (p sc) (SL.get_next n_old_empty_slabs) `star`
+      SL.llist (p sc) (SL.get_next n_empty) `star`
       vptr empty_slabs `star`
-      (p sc) (SL.get_data n_old_empty_slabs)
+      (p sc) (SL.get_data n_empty)
     );
-    SL.pack_list (p sc) empty_slabs partial_slabs (SL.get_data n_old_empty_slabs);
-    return (SL.get_next n_old_empty_slabs, empty_slabs)
+    SL.pack_list (p sc)
+      empty_slabs
+      partial_slabs
+      (SL.get_data n_empty);
+    return (snd r, (SL.get_next n_empty, empty_slabs))
   ) else (
     assert (not (SL.is_null_t partial_slabs));
-    sladmit ();
-    return (SL.null_t, SL.null_t)
+    let n_partial = SL.unpack_list (p sc) partial_slabs in
+    let h = get () in
+    let md = SL.get_data n_partial in
+    assume (has_free_slot sc (A.asel md h));
+    let r = allocate_slot_kiss sc
+      (SL.get_data n_partial)
+      (f (SL.get_data n_partial)) in
+    SL.pack_list (p sc)
+      partial_slabs
+      (SL.get_next n_partial)
+      (SL.get_data n_partial);
+    return (snd r, (partial_slabs, empty_slabs))
   )
-
-
-
-(*)
-let allocate_slab3
-  (size_class: sc)
-  (partial_slabs: SL.t (slab_metadata))
-  (empty_slabs: SL.t (slab_metadata))
-  //: Steel (SL.cell (slab_metadata))
-  : Steel unit
-  (
-  SL.llist p partial_slabs
-  `star`
-  SL.llist p empty_slabs
-  )
-  (
-  fun r ->
-  SL.llist p partial_slabs
-  `star`
-  SL.llist p empty_slabs
-  //SL.llist p (fst r)
-  //`star`
-  //SL.llist p (snd r)
-  )
-  //(fun n -> vptr slabs `star` SL.llist p (SL.get_next n) `star` p (SL.get_data n))
-  (requires fun _ ->
-    not (SL.is_null_t empty_slabs) /\
-    not (SL.is_null_t partial_slabs))
-  (ensures fun h0 _ h1 ->
-    let empty0 = SL.v_llist p empty_slabs h0 in
-    let partial0 = SL.v_llist p partial_slabs h0 in
-    assume (Cons? empty0);
-    assume (Cons? partial0);
-    SL.v_llist p empty_slabs h1 == (L.hd partial0) :: (L.tl empty0) /\
-    SL.v_llist p partial_slabs h1 == (L.hd empty0) :: (L.tl partial0))
-  =
-  let n_partial = SL.unpack_list p partial_slabs in
-  let n_empty = SL.unpack_list p empty_slabs in
-  let new_n_partial = SL.mk_cell (SL.get_next n_partial) (SL.get_data n_empty) in
-  let new_n_empty = SL.mk_cell (SL.get_next n_empty) (SL.get_data n_partial) in
-  write partial_slabs new_n_partial;
-  write empty_slabs new_n_empty;
-  SL.pack_list p partial_slabs (SL.get_next n_partial) (SL.get_data n_empty);
-  SL.pack_list p empty_slabs (SL.get_next n_empty) (SL.get_data n_partial);
-
-  return ()
-  //let v = read slabs in
-  //SL.pack_list p slabs (SL.get_next n) (SL.get_data v);
-
-
 
 (*)
 //noextract
